%----------------------------------------------------------------------------------------
% PACKAGES AND DOCUMENT CONFIGURATIONS
%----------------------------------------------------------------------------------------

\documentclass[11pt,landscape]{memoir}
\usepackage[landscape]{geometry}
\usepackage{amssymb,amsmath,verbatim,graphicx,microtype,upquote,units,booktabs,siunitx,setspace,graphicx,enumitem,siunitx,ifthen,calc,multicol,listings,xcolor}
\usepackage[absolute]{textpos}

\ifthenelse{\lengthtest {\paperwidth = 11in}}
    {\geometry{top=.1in,left=.2in,right=.2in,bottom=.1in}}
    {\ifthenelse{\lengthtest{ \paperwidth = 297mm}}
        {\geometry{top=1cm,left=1cm,right=1cm,bottom=1cm}}
        {\geometry{top=1cm,left=1cm,right=1cm,bottom=1cm}}
    }

% Change spacing between paragraphs
\setlength{\parindent}{0pt}
\setlength{\parskip}{0pt plus 0.5ex}

%---------------------------------------------------------------------------------------
% DOCUMENT INFORMATION
%----------------------------------------------------------------------------------------

\begin{document}

\begin{itemize}
    \item \textbf{Formulas}
    \item Conditional Probability: $P(e \land h) = P(e \mid h) * P(h)$
    \item Bayes' Rule: $P(e \mid h) * P(h) = P(h \mid e) * P(e)$
    \item Chain Rule: $P(a_1 \land a_2 \land a_3) = P(a_1 \mid a_2 \land a_3) * P(a_2 \mid a_3) * P(a_3)$
    \item Filtering Formula: $P(s_i \mid o_{0 \ldots i} = \frac{P(o_i \mid s_i) * \sum_{s_{i-1} \in S_{i-1}} P(s_i \mid s_{i-1}) * P(s_{i-1} \mid o_{0 \ldots 1}) * P(o_{0 \ldots i-1})}{P(o_{0 \ldots i})}$ \\
        where $P(o_{0 \ldots i})$ means $P(o_0 \land o_1 \land \cdots \land o_i)$
\end{itemize}

\begin{itemize}
    \item \textbf{Axioms of probability}
    \item $P(a) \ge 0$
    \item $P(true) = 1$
    \item $P(a \land b) = P(a) + P(b)$ if $a$ and $b$ are mutually exclusive
\end{itemize}

\begin{itemize}
    \item \textbf{Propositions}
    \item $P(\lnot a) = 1 - P(a)$
    \item $P(a) = \sum_{x \in domain(X)} P(a \land X = x)$
    \item $P(a \lor b) = P(a) + P(b) - P(a \land b)$
    \item If $a \leftrightarrow b$ then $P(a) = P(b)$
    \item $P(a) = P(a \land b) + P(a \land \lnot b) = \sum_{b \in B}(a \land b)$
\end{itemize}

\end{document}
